src/program_proof/mvcc/tuple_remove_versions.v
@@ -5,7 +5,7 @@ Context `{!heapGS Σ, !mvcc_ghostG Σ}.
 
 Lemma val_to_ver_with_val_ty (x : val) :
   val_ty x (uint64T * (boolT * (stringT * unitT))%ht) ->
-  (∃ (b : u64)  (e : bool) (v : string), x = ver_to_val (b, e, v)).
+  (∃ (b : u64)  (e : bool) (v : byte_string), x = ver_to_val (b, e, v)).
 Proof.
   intros H.
   inversion_clear H. 
