src/program_proof/tulip/encode.v
@@ -1,80 +1,14 @@
 From Perennial.program_proof Require Import grove_prelude.
 From Perennial.program_proof.tulip Require Import base.
 
-(* TODO: this really should be made general. *)
-
-Definition encode_string (x : string) : list u8 :=
-  let bs := string_to_bytes x in
-  u64_le (U64 (length bs)) ++ bs.
-
-Opaque encode_string.
-
-Definition encode_strings_step (bs : list u8) (x : string) : list u8 :=
-  bs ++ encode_string x.
-
-Definition encode_strings_xlen (xs : list string) : list u8 :=
-  foldl encode_strings_step [] xs.
-
-Definition encode_strings (xs : list string) : list u8 :=
-  u64_le (U64 (length xs)) ++ encode_strings_xlen xs.
-
-Lemma encode_strings_xlen_snoc xs x :
-  encode_strings_xlen (xs ++ [x]) = encode_strings_xlen xs ++ encode_string x.
-Proof.
-  by rewrite /encode_strings_xlen foldl_snoc /encode_strings_step.
-Qed.
-
-Lemma foldl_encode_strings_step_app (bs : list u8) (xs : list string) :
-  foldl encode_strings_step bs xs = bs ++ foldl encode_strings_step [] xs.
-Proof.
-  generalize dependent bs.
-  induction xs as [| x xs IH]; intros bs.
-  { by rewrite /= app_nil_r. }
-  rewrite /= (IH (encode_strings_step bs x)) (IH (encode_strings_step [] x)).
-  rewrite {1 3}/encode_strings_step.
-  by rewrite app_nil_l app_assoc.
-Qed.
-
-Lemma encode_strings_xlen_cons xs x :
-  encode_strings_xlen (x :: xs) = encode_string x ++ encode_strings_xlen xs.
-Proof.
-  rewrite /encode_strings_xlen /= foldl_encode_strings_step_app.
-  by rewrite {1}/encode_strings_step app_nil_l.
-Qed.
-
-Lemma encode_strings_xlen_length_inv xs n :
-  (length (encode_strings_xlen xs) ≤ n)%nat ->
-  (length xs ≤ n)%nat.
-Proof.
-  generalize dependent n.
-  induction xs as [| x xs IH]; intros n; first done.
-  rewrite encode_strings_xlen_cons length_app /=.
-  assert (length (encode_string x) ≠ O).
-  { by destruct (nil_or_length_pos (encode_string x)). }
-  intros Hlen.
-  assert (Hlenxs : (length xs ≤ pred n)%nat).
-  { apply IH. lia. }
-  lia.
-Qed.
-
-Lemma encode_strings_length_inv xs n :
-  (length (encode_strings xs) ≤ n)%nat ->
-  (length xs ≤ n)%nat.
-Proof.
-  rewrite /encode_strings length_app.
-  intros Hn.
-  pose proof (encode_strings_xlen_length_inv xs n) as Hlen.
-  lia.
-Qed.
-
 Definition encode_dbval (x : dbval) : list u8 :=
   match x with
-  | Some v => [U8 1] ++ encode_string v
+  | Some v => [U8 1] ++ v
   | None => [U8 0]
   end.
 
 Definition encode_dbmod (x : dbmod) : list u8 :=
-  encode_string x.1 ++ encode_dbval x.2.
+  x.1 ++ encode_dbval x.2.
 
 Definition encode_dbmods_step (bs : list u8) (x : dbmod) : list u8 :=
   bs ++ encode_dbmod x.
@@ -117,7 +51,7 @@ Proof.
   induction xs as [| x xs IH]; intros n; first done.
   rewrite encode_dbmods_xlen_cons length_app /=.
   assert (length (encode_dbmod x) ≠ O).
-  { by destruct (nil_or_length_pos (encode_dbmod x)). }
+  { by destruct x as [[] []]. }
   intros Hlen.
   assert (Hlenxs : (length xs ≤ pred n)%nat).
   { apply IH. lia. }
